src3.0/Transforms/alive_alloca.v
@@ -139,8 +139,8 @@ Proof.
   eapply H0 in Hlkpa; eauto. clear H0.
   eapply H in Hlkpa'; eauto.
   destruct Hlkpa' as [J1 J2].
-  destruct J1 as [[mb [J1 [J3 J4]]] _]; subst.
-  eapply NoDup_disjoint in H1; eauto.
+  destruct J1 as [_ [[mb [J1 [J3 J4]]] _]]; subst.
+  eapply alist.NoDup_disjoint in H1; eauto.
   eapply free_allocas_preserves_mload; eauto.
 Qed.
 
